lib/ssr_list_utils.v
@@ -4,6 +4,10 @@ Require Import ssreflect ssrfun ssrbool eqtype seq.
 
 Set Bullet Behavior "Strict Subproofs".
 
+Theorem eq_op_is_equiv_dec (T : eqType) (x y : T) :
+  x == y = SetoidDec.equiv_dec x y.
+Proof. by case: (SetoidDec.equiv_dec _ _) => /= ?; apply/eqP. Qed.
+
 Theorem inP (T : eqType) (x : T) (xs : seq T) : reflect (In x xs) (x \in xs).
 Proof.
   case B: (x \in xs); constructor; move: B.
@@ -33,30 +37,14 @@ Proof.
     by move/inP in NIN.
 Qed.
 
-Lemma mem_rem_weaken (T : eqType) (x y : T) (xs : seq T) :
-  x \in rem y xs -> x \in xs.
-Proof.
-  elim: xs => [// | /= x' xs' IH]; rewrite inE.
-  case (x' == y).
-  - by move=> REM; rewrite REM orbT.
-  - rewrite inE; move=> /orP [EQ | IN].
-    + by rewrite EQ.
-    + by apply IH in IN; rewrite IN orbT.
-Qed.
-       
-Theorem in2_rem (T : eqType) (a b y : T) (xs : seq T) :
-  In2 a b (rem y xs) -> In2 a b xs.
-Proof.
-  elim: xs=> [// | /= x xs' IH].
-  case E: (x == y) => IN2; move/eqP: E; [move=> ?; subst | move=> NEQ].
-  - by apply In2_there.
-  - inversion IN2 as [rem_xs' IN | rem_xs' IN | x' rem_xs' IN2']; subst.
-    + by apply In2_here_1;
-         move/inP in IN; apply mem_rem_weaken in IN; apply /inP.
-    + by apply In2_here_2;
-         move/inP in IN; apply mem_rem_weaken in IN; apply /inP.
-    + by apply In2_there, IH.
-Qed.
-
 Definition rem_all {T : eqType} : T -> seq T -> seq T :=
   filter \o predC1.
+
+Theorem rem_all_is_delete (T : eqType) (a : T) (xs : seq T) :
+  rem_all a xs = delete a xs.
+Proof.
+  rewrite /rem_all /delete.
+  elim: xs => [// | /= x xs' IH].
+  rewrite eq_sym eq_op_is_equiv_dec.
+  by case: (SetoidDec.equiv_dec _ _) => /=; rewrite IH.
+Qed.
